Most vectors pass

TestVectorsAwsCryptographicMaterialProviders/runtimes/java/src/main/smithy-generated/software/amazon/cryptography/materialProviders/wrapped/keys/KeyVectors.java
@@ -1,0 +1,110 @@
+// Copyright Amazon.com Inc. or its affiliates. All Rights Reserved.
+// SPDX-License-Identifier: Apache-2.0
+// Do not modify this file. This file is machine generated, and any changes to it will be overwritten.
+package software.amazon.cryptography.materialProviders.wrapped.keys;
+
+import Dafny.Aws.Cryptography.MaterialProviders.Wrapped.Keys.KeyVectorsClient;
+import Dafny.Aws.Cryptography.MaterialProviders.Wrapped.Keys.Types.Error;
+import Dafny.Aws.Cryptography.MaterialProviders.Wrapped.Keys.Types.IKeyVectorsClient;
+import Dafny.Aws.Cryptography.MaterialProviders.Wrapped.Keys.__default;
+import Wrappers_Compile.Result;
+import java.lang.IllegalArgumentException;
+import java.util.Objects;
+import software.amazon.cryptography.materialProviders.IKeyring;
+import software.amazon.cryptography.materialProviders.Keyring;
+import software.amazon.cryptography.materialProviders.wrapped.keys.model.GetKeyDescriptionInput;
+import software.amazon.cryptography.materialProviders.wrapped.keys.model.GetKeyDescriptionOutput;
+import software.amazon.cryptography.materialProviders.wrapped.keys.model.KeyVectorsConfig;
+import software.amazon.cryptography.materialProviders.wrapped.keys.model.SerializeKeyDescriptionInput;
+import software.amazon.cryptography.materialProviders.wrapped.keys.model.SerializeKeyDescriptionOutput;
+import software.amazon.cryptography.materialProviders.wrapped.keys.model.TestVectorKeyringInput;
+
+public class KeyVectors {
+  private final IKeyVectorsClient _impl;
+
+  protected KeyVectors(BuilderImpl builder) {
+    KeyVectorsConfig nativeValue = builder.KeyVectorsConfig();
+    Dafny.Aws.Cryptography.MaterialProviders.Wrapped.Keys.Types.KeyVectorsConfig dafnyValue = ToDafny.KeyVectorsConfig(nativeValue);
+    Result<KeyVectorsClient, Error> result = __default.KeyVectors(dafnyValue);
+    if (result.is_Failure()) {
+      throw ToNative.Error(result.dtor_error());
+    }
+    this._impl = result.dtor_value();
+  }
+
+  public static Builder builder() {
+    return new BuilderImpl();
+  }
+
+  public IKeyring CreateTestVectorKeyring(TestVectorKeyringInput nativeValue) {
+    Dafny.Aws.Cryptography.MaterialProviders.Wrapped.Keys.Types.TestVectorKeyringInput dafnyValue = ToDafny.TestVectorKeyringInput(nativeValue);
+    Result<Dafny.Aws.Cryptography.MaterialProviders.Types.IKeyring, Error> result = this._impl.CreateTestVectorKeyring(dafnyValue);
+    if (result.is_Failure()) {
+      throw ToNative.Error(result.dtor_error());
+    }
+    return Keyring.wrap(result.dtor_value());
+  }
+
+  public IKeyring CreateWappedTestVectorKeyring(TestVectorKeyringInput nativeValue) {
+    Dafny.Aws.Cryptography.MaterialProviders.Wrapped.Keys.Types.TestVectorKeyringInput dafnyValue = ToDafny.TestVectorKeyringInput(nativeValue);
+    Result<Dafny.Aws.Cryptography.MaterialProviders.Types.IKeyring, Error> result = this._impl.CreateWappedTestVectorKeyring(dafnyValue);
+    if (result.is_Failure()) {
+      throw ToNative.Error(result.dtor_error());
+    }
+    return Keyring.wrap(result.dtor_value());
+  }
+
+  public GetKeyDescriptionOutput GetKeyDescription(GetKeyDescriptionInput nativeValue) {
+    Dafny.Aws.Cryptography.MaterialProviders.Wrapped.Keys.Types.GetKeyDescriptionInput dafnyValue = ToDafny.GetKeyDescriptionInput(nativeValue);
+    Result<Dafny.Aws.Cryptography.MaterialProviders.Wrapped.Keys.Types.GetKeyDescriptionOutput, Error> result = this._impl.GetKeyDescription(dafnyValue);
+    if (result.is_Failure()) {
+      throw ToNative.Error(result.dtor_error());
+    }
+    return ToNative.GetKeyDescriptionOutput(result.dtor_value());
+  }
+
+  public SerializeKeyDescriptionOutput SerializeKeyDescription(
+      SerializeKeyDescriptionInput nativeValue) {
+    Dafny.Aws.Cryptography.MaterialProviders.Wrapped.Keys.Types.SerializeKeyDescriptionInput dafnyValue = ToDafny.SerializeKeyDescriptionInput(nativeValue);
+    Result<Dafny.Aws.Cryptography.MaterialProviders.Wrapped.Keys.Types.SerializeKeyDescriptionOutput, Error> result = this._impl.SerializeKeyDescription(dafnyValue);
+    if (result.is_Failure()) {
+      throw ToNative.Error(result.dtor_error());
+    }
+    return ToNative.SerializeKeyDescriptionOutput(result.dtor_value());
+  }
+
+  protected IKeyVectorsClient impl() {
+    return this._impl;
+  }
+
+  public interface Builder {
+    Builder KeyVectorsConfig(KeyVectorsConfig KeyVectorsConfig);
+
+    KeyVectorsConfig KeyVectorsConfig();
+
+    KeyVectors build();
+  }
+
+  static class BuilderImpl implements Builder {
+    protected KeyVectorsConfig KeyVectorsConfig;
+
+    protected BuilderImpl() {
+    }
+
+    public Builder KeyVectorsConfig(KeyVectorsConfig KeyVectorsConfig) {
+      this.KeyVectorsConfig = KeyVectorsConfig;
+      return this;
+    }
+
+    public KeyVectorsConfig KeyVectorsConfig() {
+      return this.KeyVectorsConfig;
+    }
+
+    public KeyVectors build() {
+      if (Objects.isNull(this.KeyVectorsConfig()))  {
+        throw new IllegalArgumentException("Missing value for required field `KeyVectorsConfig`");
+      }
+      return new KeyVectors(this);
+    }
+  }
+}
