TestVectorsAwsCryptographicMaterialProviders/runtimes/java/src/main/smithy-generated/software/amazon/cryptography/materialProviders/wrapped/keys/ToDafny.java
@@ -1,0 +1,184 @@
+// Copyright Amazon.com Inc. or its affiliates. All Rights Reserved.
+// SPDX-License-Identifier: Apache-2.0
+// Do not modify this file. This file is machine generated, and any changes to it will be overwritten.
+package software.amazon.cryptography.materialProviders.wrapped.keys;
+
+import Dafny.Aws.Cryptography.MaterialProviders.Types.DiscoveryFilter;
+import Dafny.Aws.Cryptography.MaterialProviders.Types.PaddingScheme;
+import Dafny.Aws.Cryptography.MaterialProviders.Wrapped.Keys.Types.Error;
+import Dafny.Aws.Cryptography.MaterialProviders.Wrapped.Keys.Types.Error_KeyVectorException;
+import Dafny.Aws.Cryptography.MaterialProviders.Wrapped.Keys.Types.GetKeyDescriptionInput;
+import Dafny.Aws.Cryptography.MaterialProviders.Wrapped.Keys.Types.GetKeyDescriptionOutput;
+import Dafny.Aws.Cryptography.MaterialProviders.Wrapped.Keys.Types.InvalidKeyring;
+import Dafny.Aws.Cryptography.MaterialProviders.Wrapped.Keys.Types.KMSInfo;
+import Dafny.Aws.Cryptography.MaterialProviders.Wrapped.Keys.Types.KeyDescription;
+import Dafny.Aws.Cryptography.MaterialProviders.Wrapped.Keys.Types.KeyVectorsConfig;
+import Dafny.Aws.Cryptography.MaterialProviders.Wrapped.Keys.Types.KmsMrkAware;
+import Dafny.Aws.Cryptography.MaterialProviders.Wrapped.Keys.Types.KmsMrkAwareDiscovery;
+import Dafny.Aws.Cryptography.MaterialProviders.Wrapped.Keys.Types.RawAES;
+import Dafny.Aws.Cryptography.MaterialProviders.Wrapped.Keys.Types.RawRSA;
+import Dafny.Aws.Cryptography.MaterialProviders.Wrapped.Keys.Types.SerializeKeyDescriptionInput;
+import Dafny.Aws.Cryptography.MaterialProviders.Wrapped.Keys.Types.SerializeKeyDescriptionOutput;
+import Dafny.Aws.Cryptography.MaterialProviders.Wrapped.Keys.Types.TestVectorKeyringInput;
+import Wrappers_Compile.Option;
+import dafny.DafnySequence;
+import java.lang.Byte;
+import java.lang.Character;
+import java.lang.IllegalArgumentException;
+import java.lang.RuntimeException;
+import java.util.Objects;
+import software.amazon.cryptography.materialProviders.wrapped.keys.model.CollectionOfErrors;
+import software.amazon.cryptography.materialProviders.wrapped.keys.model.KeyVectorException;
+import software.amazon.cryptography.materialProviders.wrapped.keys.model.OpaqueError;
+
+public class ToDafny {
+  public static Error Error(RuntimeException nativeValue) {
+    if (nativeValue instanceof KeyVectorException) {
+      return ToDafny.Error((KeyVectorException) nativeValue);
+    }
+    if (nativeValue instanceof OpaqueError) {
+      return ToDafny.Error((OpaqueError) nativeValue);
+    }
+    if (nativeValue instanceof CollectionOfErrors) {
+      return ToDafny.Error((CollectionOfErrors) nativeValue);
+    }
+    return Error.create_Opaque(nativeValue);
+  }
+
+  public static Error Error(OpaqueError nativeValue) {
+    return Error.create_Opaque(nativeValue.obj());
+  }
+
+  public static Error Error(CollectionOfErrors nativeValue) {
+    DafnySequence<? extends Error> list = software.amazon.dafny.conversion.ToDafny.Aggregate.GenericToSequence(
+        nativeValue.list(), 
+        ToDafny::Error, 
+        Error._typeDescriptor());
+    return Error.create_CollectionOfErrors(list);
+  }
+
+  public static GetKeyDescriptionOutput GetKeyDescriptionOutput(
+      software.amazon.cryptography.materialProviders.wrapped.keys.model.GetKeyDescriptionOutput nativeValue) {
+    KeyDescription keyDescription;
+    keyDescription = ToDafny.KeyDescription(nativeValue.keyDescription());
+    return new GetKeyDescriptionOutput(keyDescription);
+  }
+
+  public static TestVectorKeyringInput TestVectorKeyringInput(
+      software.amazon.cryptography.materialProviders.wrapped.keys.model.TestVectorKeyringInput nativeValue) {
+    KeyDescription keyDescription;
+    keyDescription = ToDafny.KeyDescription(nativeValue.keyDescription());
+    return new TestVectorKeyringInput(keyDescription);
+  }
+
+  public static SerializeKeyDescriptionOutput SerializeKeyDescriptionOutput(
+      software.amazon.cryptography.materialProviders.wrapped.keys.model.SerializeKeyDescriptionOutput nativeValue) {
+    DafnySequence<? extends Byte> json;
+    json = software.amazon.dafny.conversion.ToDafny.Simple.ByteSequence(nativeValue.json());
+    return new SerializeKeyDescriptionOutput(json);
+  }
+
+  public static SerializeKeyDescriptionInput SerializeKeyDescriptionInput(
+      software.amazon.cryptography.materialProviders.wrapped.keys.model.SerializeKeyDescriptionInput nativeValue) {
+    KeyDescription keyDescription;
+    keyDescription = ToDafny.KeyDescription(nativeValue.keyDescription());
+    return new SerializeKeyDescriptionInput(keyDescription);
+  }
+
+  public static KmsMrkAwareDiscovery KmsMrkAwareDiscovery(
+      software.amazon.cryptography.materialProviders.wrapped.keys.model.KmsMrkAwareDiscovery nativeValue) {
+    DafnySequence<? extends Character> keyId;
+    keyId = software.amazon.dafny.conversion.ToDafny.Simple.CharacterSequence(nativeValue.keyId());
+    DafnySequence<? extends Character> defaultMrkRegion;
+    defaultMrkRegion = software.amazon.dafny.conversion.ToDafny.Simple.CharacterSequence(nativeValue.defaultMrkRegion());
+    Option<DiscoveryFilter> awsKmsDiscoveryFilter;
+    awsKmsDiscoveryFilter = Objects.nonNull(nativeValue.awsKmsDiscoveryFilter()) ?
+        Option.create_Some(software.amazon.cryptography.materialProviders.ToDafny.DiscoveryFilter(nativeValue.awsKmsDiscoveryFilter()))
+        : Option.create_None();
+    return new KmsMrkAwareDiscovery(keyId, defaultMrkRegion, awsKmsDiscoveryFilter);
+  }
+
+  public static KmsMrkAware KmsMrkAware(
+      software.amazon.cryptography.materialProviders.wrapped.keys.model.KmsMrkAware nativeValue) {
+    DafnySequence<? extends Character> keyId;
+    keyId = software.amazon.dafny.conversion.ToDafny.Simple.CharacterSequence(nativeValue.keyId());
+    return new KmsMrkAware(keyId);
+  }
+
+  public static GetKeyDescriptionInput GetKeyDescriptionInput(
+      software.amazon.cryptography.materialProviders.wrapped.keys.model.GetKeyDescriptionInput nativeValue) {
+    DafnySequence<? extends Byte> json;
+    json = software.amazon.dafny.conversion.ToDafny.Simple.ByteSequence(nativeValue.json());
+    return new GetKeyDescriptionInput(json);
+  }
+
+  public static RawAES RawAES(
+      software.amazon.cryptography.materialProviders.wrapped.keys.model.RawAES nativeValue) {
+    DafnySequence<? extends Character> keyId;
+    keyId = software.amazon.dafny.conversion.ToDafny.Simple.CharacterSequence(nativeValue.keyId());
+    DafnySequence<? extends Character> providerId;
+    providerId = software.amazon.dafny.conversion.ToDafny.Simple.CharacterSequence(nativeValue.providerId());
+    return new RawAES(keyId, providerId);
+  }
+
+  public static KeyVectorsConfig KeyVectorsConfig(
+      software.amazon.cryptography.materialProviders.wrapped.keys.model.KeyVectorsConfig nativeValue) {
+    DafnySequence<? extends Character> keyManifiestPath;
+    keyManifiestPath = software.amazon.dafny.conversion.ToDafny.Simple.CharacterSequence(nativeValue.keyManifiestPath());
+    return new KeyVectorsConfig(keyManifiestPath);
+  }
+
+  public static RawRSA RawRSA(
+      software.amazon.cryptography.materialProviders.wrapped.keys.model.RawRSA nativeValue) {
+    DafnySequence<? extends Character> keyId;
+    keyId = software.amazon.dafny.conversion.ToDafny.Simple.CharacterSequence(nativeValue.keyId());
+    DafnySequence<? extends Character> providerId;
+    providerId = software.amazon.dafny.conversion.ToDafny.Simple.CharacterSequence(nativeValue.providerId());
+    PaddingScheme padding;
+    padding = software.amazon.cryptography.materialProviders.ToDafny.PaddingScheme(nativeValue.padding());
+    return new RawRSA(keyId, providerId, padding);
+  }
+
+  public static InvalidKeyring InvalidKeyring(
+      software.amazon.cryptography.materialProviders.wrapped.keys.model.InvalidKeyring nativeValue) {
+    DafnySequence<? extends Character> keyId;
+    keyId = software.amazon.dafny.conversion.ToDafny.Simple.CharacterSequence(nativeValue.keyId());
+    return new InvalidKeyring(keyId);
+  }
+
+  public static KMSInfo KMSInfo(
+      software.amazon.cryptography.materialProviders.wrapped.keys.model.KMSInfo nativeValue) {
+    DafnySequence<? extends Character> keyId;
+    keyId = software.amazon.dafny.conversion.ToDafny.Simple.CharacterSequence(nativeValue.keyId());
+    return new KMSInfo(keyId);
+  }
+
+  public static Error Error(KeyVectorException nativeValue) {
+    DafnySequence<? extends Character> message;
+    message = software.amazon.dafny.conversion.ToDafny.Simple.CharacterSequence(nativeValue.message());
+    return new Error_KeyVectorException(message);
+  }
+
+  public static KeyDescription KeyDescription(
+      software.amazon.cryptography.materialProviders.wrapped.keys.model.KeyDescription nativeValue) {
+    if (Objects.nonNull(nativeValue.Kms())) {
+      return KeyDescription.create_Kms(ToDafny.KMSInfo(nativeValue.Kms()));
+    }
+    if (Objects.nonNull(nativeValue.KmsMrk())) {
+      return KeyDescription.create_KmsMrk(ToDafny.KmsMrkAware(nativeValue.KmsMrk()));
+    }
+    if (Objects.nonNull(nativeValue.KmsMrkDiscovery())) {
+      return KeyDescription.create_KmsMrkDiscovery(ToDafny.KmsMrkAwareDiscovery(nativeValue.KmsMrkDiscovery()));
+    }
+    if (Objects.nonNull(nativeValue.RSA())) {
+      return KeyDescription.create_RSA(ToDafny.RawRSA(nativeValue.RSA()));
+    }
+    if (Objects.nonNull(nativeValue.AES())) {
+      return KeyDescription.create_AES(ToDafny.RawAES(nativeValue.AES()));
+    }
+    if (Objects.nonNull(nativeValue.Invalid())) {
+      return KeyDescription.create_Invalid(ToDafny.InvalidKeyring(nativeValue.Invalid()));
+    }
+    throw new IllegalArgumentException("Cannot convert " + nativeValue + " to Dafny.Aws.Cryptography.MaterialProviders.Wrapped.Keys.Types.KeyDescription.");
+  }
+}
