TestVectorsAwsCryptographicMaterialProviders/runtimes/java/src/main/smithy-generated/software/amazon/cryptography/materialProviders/wrapped/keys/model/KeyDescription.java
@@ -1,0 +1,190 @@
+// Copyright Amazon.com Inc. or its affiliates. All Rights Reserved.
+// SPDX-License-Identifier: Apache-2.0
+// Do not modify this file. This file is machine generated, and any changes to it will be overwritten.
+package software.amazon.cryptography.materialProviders.wrapped.keys.model;
+
+import java.util.Objects;
+
+public class KeyDescription {
+  private final KMSInfo Kms;
+
+  private final KmsMrkAware KmsMrk;
+
+  private final KmsMrkAwareDiscovery KmsMrkDiscovery;
+
+  private final RawRSA RSA;
+
+  private final RawAES AES;
+
+  private final InvalidKeyring Invalid;
+
+  protected KeyDescription(BuilderImpl builder) {
+    this.Kms = builder.Kms();
+    this.KmsMrk = builder.KmsMrk();
+    this.KmsMrkDiscovery = builder.KmsMrkDiscovery();
+    this.RSA = builder.RSA();
+    this.AES = builder.AES();
+    this.Invalid = builder.Invalid();
+  }
+
+  public KMSInfo Kms() {
+    return this.Kms;
+  }
+
+  public KmsMrkAware KmsMrk() {
+    return this.KmsMrk;
+  }
+
+  public KmsMrkAwareDiscovery KmsMrkDiscovery() {
+    return this.KmsMrkDiscovery;
+  }
+
+  public RawRSA RSA() {
+    return this.RSA;
+  }
+
+  public RawAES AES() {
+    return this.AES;
+  }
+
+  public InvalidKeyring Invalid() {
+    return this.Invalid;
+  }
+
+  public Builder toBuilder() {
+    return new BuilderImpl(this);
+  }
+
+  public static Builder builder() {
+    return new BuilderImpl();
+  }
+
+  public interface Builder {
+    Builder Kms(KMSInfo Kms);
+
+    KMSInfo Kms();
+
+    Builder KmsMrk(KmsMrkAware KmsMrk);
+
+    KmsMrkAware KmsMrk();
+
+    Builder KmsMrkDiscovery(KmsMrkAwareDiscovery KmsMrkDiscovery);
+
+    KmsMrkAwareDiscovery KmsMrkDiscovery();
+
+    Builder RSA(RawRSA RSA);
+
+    RawRSA RSA();
+
+    Builder AES(RawAES AES);
+
+    RawAES AES();
+
+    Builder Invalid(InvalidKeyring Invalid);
+
+    InvalidKeyring Invalid();
+
+    KeyDescription build();
+  }
+
+  static class BuilderImpl implements Builder {
+    protected KMSInfo Kms;
+
+    protected KmsMrkAware KmsMrk;
+
+    protected KmsMrkAwareDiscovery KmsMrkDiscovery;
+
+    protected RawRSA RSA;
+
+    protected RawAES AES;
+
+    protected InvalidKeyring Invalid;
+
+    protected BuilderImpl() {
+    }
+
+    protected BuilderImpl(KeyDescription model) {
+      this.Kms = model.Kms();
+      this.KmsMrk = model.KmsMrk();
+      this.KmsMrkDiscovery = model.KmsMrkDiscovery();
+      this.RSA = model.RSA();
+      this.AES = model.AES();
+      this.Invalid = model.Invalid();
+    }
+
+    public Builder Kms(KMSInfo Kms) {
+      this.Kms = Kms;
+      return this;
+    }
+
+    public KMSInfo Kms() {
+      return this.Kms;
+    }
+
+    public Builder KmsMrk(KmsMrkAware KmsMrk) {
+      this.KmsMrk = KmsMrk;
+      return this;
+    }
+
+    public KmsMrkAware KmsMrk() {
+      return this.KmsMrk;
+    }
+
+    public Builder KmsMrkDiscovery(KmsMrkAwareDiscovery KmsMrkDiscovery) {
+      this.KmsMrkDiscovery = KmsMrkDiscovery;
+      return this;
+    }
+
+    public KmsMrkAwareDiscovery KmsMrkDiscovery() {
+      return this.KmsMrkDiscovery;
+    }
+
+    public Builder RSA(RawRSA RSA) {
+      this.RSA = RSA;
+      return this;
+    }
+
+    public RawRSA RSA() {
+      return this.RSA;
+    }
+
+    public Builder AES(RawAES AES) {
+      this.AES = AES;
+      return this;
+    }
+
+    public RawAES AES() {
+      return this.AES;
+    }
+
+    public Builder Invalid(InvalidKeyring Invalid) {
+      this.Invalid = Invalid;
+      return this;
+    }
+
+    public InvalidKeyring Invalid() {
+      return this.Invalid;
+    }
+
+    public KeyDescription build() {
+      if (!onlyOneNonNull()) {
+        throw new IllegalArgumentException("`KeyDescription` is a Union. A Union MUST have one and only one value set.");
+      }
+      return new KeyDescription(this);
+    }
+
+    private boolean onlyOneNonNull() {
+      Object[] allValues = {this.Kms, this.KmsMrk, this.KmsMrkDiscovery, this.RSA, this.AES, this.Invalid};
+      boolean haveOneNonNull = false;
+      for (Object o : allValues) {
+        if (Objects.nonNull(o)) {
+          if (haveOneNonNull) {
+            return false;
+          }
+          haveOneNonNull = true;
+        }
+      }
+      return haveOneNonNull;
+    }
+  }
+}
