TestVectorsAwsCryptographicMaterialProviders/runtimes/net/Generated/KeyVectors/KeyDescription.cs
@@ -1,0 +1,68 @@
+// Copyright Amazon.com Inc. or its affiliates. All Rights Reserved.
+// SPDX-License-Identifier: Apache-2.0
+// Do not modify this file. This file is machine generated, and any changes to it will be overwritten.
+using System;
+ using AWS.Cryptography.MaterialProviders.Wrapped.Keys; namespace AWS.Cryptography.MaterialProviders.Wrapped.Keys {
+ public class KeyDescription {
+ private AWS.Cryptography.MaterialProviders.Wrapped.Keys.KMSInfo _kms ;
+ private AWS.Cryptography.MaterialProviders.Wrapped.Keys.KmsMrkAware _kmsMrk ;
+ private AWS.Cryptography.MaterialProviders.Wrapped.Keys.KmsMrkAwareDiscovery _kmsMrkDiscovery ;
+ private AWS.Cryptography.MaterialProviders.Wrapped.Keys.RawRSA _rSA ;
+ private AWS.Cryptography.MaterialProviders.Wrapped.Keys.RawAES _aES ;
+ private AWS.Cryptography.MaterialProviders.Wrapped.Keys.InvalidKeyring _invalid ;
+ public AWS.Cryptography.MaterialProviders.Wrapped.Keys.KMSInfo Kms {
+ get { return this._kms; }
+ set { this._kms = value; }
+}
+ public bool IsSetKms () {
+ return this._kms != null;
+}
+ public AWS.Cryptography.MaterialProviders.Wrapped.Keys.KmsMrkAware KmsMrk {
+ get { return this._kmsMrk; }
+ set { this._kmsMrk = value; }
+}
+ public bool IsSetKmsMrk () {
+ return this._kmsMrk != null;
+}
+ public AWS.Cryptography.MaterialProviders.Wrapped.Keys.KmsMrkAwareDiscovery KmsMrkDiscovery {
+ get { return this._kmsMrkDiscovery; }
+ set { this._kmsMrkDiscovery = value; }
+}
+ public bool IsSetKmsMrkDiscovery () {
+ return this._kmsMrkDiscovery != null;
+}
+ public AWS.Cryptography.MaterialProviders.Wrapped.Keys.RawRSA RSA {
+ get { return this._rSA; }
+ set { this._rSA = value; }
+}
+ public bool IsSetRSA () {
+ return this._rSA != null;
+}
+ public AWS.Cryptography.MaterialProviders.Wrapped.Keys.RawAES AES {
+ get { return this._aES; }
+ set { this._aES = value; }
+}
+ public bool IsSetAES () {
+ return this._aES != null;
+}
+ public AWS.Cryptography.MaterialProviders.Wrapped.Keys.InvalidKeyring Invalid {
+ get { return this._invalid; }
+ set { this._invalid = value; }
+}
+ public bool IsSetInvalid () {
+ return this._invalid != null;
+}
+ public void Validate() {
+ var numberOfPropertiesSet = Convert.ToUInt16(IsSetKms()) +
+ Convert.ToUInt16(IsSetKmsMrk()) +
+ Convert.ToUInt16(IsSetKmsMrkDiscovery()) +
+ Convert.ToUInt16(IsSetRSA()) +
+ Convert.ToUInt16(IsSetAES()) +
+ Convert.ToUInt16(IsSetInvalid()) ;
+ if (numberOfPropertiesSet == 0) throw new System.ArgumentException("No union value set");
+
+ if (numberOfPropertiesSet > 1) throw new System.ArgumentException("Multiple union values set");
+
+}
+}
+}
