TestVectorsAwsCryptographicMaterialProviders/runtimes/net/Generated/KeyVectors/KeyVectorException.cs
@@ -1,0 +1,9 @@
+// Copyright Amazon.com Inc. or its affiliates. All Rights Reserved.
+// SPDX-License-Identifier: Apache-2.0
+// Do not modify this file. This file is machine generated, and any changes to it will be overwritten.
+using System;
+ using AWS.Cryptography.MaterialProviders.Wrapped.Keys; namespace AWS.Cryptography.MaterialProviders.Wrapped.Keys {
+ public class KeyVectorException : Exception {
+ public KeyVectorException(string message) : base(message) {}
+}
+}
