TestVectorsAwsCryptographicMaterialProviders/runtimes/net/Generated/KeyVectors/KeyVectors.cs
@@ -1,0 +1,43 @@
+// Copyright Amazon.com Inc. or its affiliates. All Rights Reserved.
+// SPDX-License-Identifier: Apache-2.0
+// Do not modify this file. This file is machine generated, and any changes to it will be overwritten.
+using System;
+ using System.IO;
+ using System.Collections.Generic;
+ using AWS.Cryptography.MaterialProviders.Wrapped.Keys;
+ using Dafny.Aws.Cryptography.MaterialProviders.Wrapped.Keys.Types; namespace AWS.Cryptography.MaterialProviders.Wrapped.Keys {
+ public class KeyVectors {
+ private readonly Dafny.Aws.Cryptography.MaterialProviders.Wrapped.Keys.Types.IKeyVectorsClient _impl;
+ public KeyVectors(AWS.Cryptography.MaterialProviders.Wrapped.Keys.KeyVectorsConfig input)
+ {
+ Dafny.Aws.Cryptography.MaterialProviders.Wrapped.Keys.Types._IKeyVectorsConfig internalInput = TypeConversion.ToDafny_N3_aws__N12_cryptography__N17_materialProviders__N7_wrapped__N4_keys__S16_KeyVectorsConfig(input);
+ var result = Dafny.Aws.Cryptography.MaterialProviders.Wrapped.Keys.__default.KeyVectors(internalInput);
+ if (result.is_Failure) throw TypeConversion.FromDafny_CommonError(result.dtor_error);
+ this._impl = result.dtor_value;
+}
+ public AWS.Cryptography.MaterialProviders.IKeyring CreateTestVectorKeyring(AWS.Cryptography.MaterialProviders.Wrapped.Keys.TestVectorKeyringInput input) {
+ Dafny.Aws.Cryptography.MaterialProviders.Wrapped.Keys.Types._ITestVectorKeyringInput internalInput = TypeConversion.ToDafny_N3_aws__N12_cryptography__N17_materialProviders__N7_wrapped__N4_keys__S22_TestVectorKeyringInput(input);
+ Wrappers_Compile._IResult<Dafny.Aws.Cryptography.MaterialProviders.Types.IKeyring, Dafny.Aws.Cryptography.MaterialProviders.Wrapped.Keys.Types._IError> result = _impl.CreateTestVectorKeyring(internalInput);
+ if (result.is_Failure) throw TypeConversion.FromDafny_CommonError(result.dtor_error);
+ return TypeConversion.FromDafny_N3_aws__N12_cryptography__N17_materialProviders__S19_CreateKeyringOutput(result.dtor_value);
+}
+ public AWS.Cryptography.MaterialProviders.IKeyring CreateWappedTestVectorKeyring(AWS.Cryptography.MaterialProviders.Wrapped.Keys.TestVectorKeyringInput input) {
+ Dafny.Aws.Cryptography.MaterialProviders.Wrapped.Keys.Types._ITestVectorKeyringInput internalInput = TypeConversion.ToDafny_N3_aws__N12_cryptography__N17_materialProviders__N7_wrapped__N4_keys__S22_TestVectorKeyringInput(input);
+ Wrappers_Compile._IResult<Dafny.Aws.Cryptography.MaterialProviders.Types.IKeyring, Dafny.Aws.Cryptography.MaterialProviders.Wrapped.Keys.Types._IError> result = _impl.CreateWappedTestVectorKeyring(internalInput);
+ if (result.is_Failure) throw TypeConversion.FromDafny_CommonError(result.dtor_error);
+ return TypeConversion.FromDafny_N3_aws__N12_cryptography__N17_materialProviders__S19_CreateKeyringOutput(result.dtor_value);
+}
+ public AWS.Cryptography.MaterialProviders.Wrapped.Keys.GetKeyDescriptionOutput GetKeyDescription(AWS.Cryptography.MaterialProviders.Wrapped.Keys.GetKeyDescriptionInput input) {
+ Dafny.Aws.Cryptography.MaterialProviders.Wrapped.Keys.Types._IGetKeyDescriptionInput internalInput = TypeConversion.ToDafny_N3_aws__N12_cryptography__N17_materialProviders__N7_wrapped__N4_keys__S22_GetKeyDescriptionInput(input);
+ Wrappers_Compile._IResult<Dafny.Aws.Cryptography.MaterialProviders.Wrapped.Keys.Types._IGetKeyDescriptionOutput, Dafny.Aws.Cryptography.MaterialProviders.Wrapped.Keys.Types._IError> result = _impl.GetKeyDescription(internalInput);
+ if (result.is_Failure) throw TypeConversion.FromDafny_CommonError(result.dtor_error);
+ return TypeConversion.FromDafny_N3_aws__N12_cryptography__N17_materialProviders__N7_wrapped__N4_keys__S23_GetKeyDescriptionOutput(result.dtor_value);
+}
+ public AWS.Cryptography.MaterialProviders.Wrapped.Keys.SerializeKeyDescriptionOutput SerializeKeyDescription(AWS.Cryptography.MaterialProviders.Wrapped.Keys.SerializeKeyDescriptionInput input) {
+ Dafny.Aws.Cryptography.MaterialProviders.Wrapped.Keys.Types._ISerializeKeyDescriptionInput internalInput = TypeConversion.ToDafny_N3_aws__N12_cryptography__N17_materialProviders__N7_wrapped__N4_keys__S28_SerializeKeyDescriptionInput(input);
+ Wrappers_Compile._IResult<Dafny.Aws.Cryptography.MaterialProviders.Wrapped.Keys.Types._ISerializeKeyDescriptionOutput, Dafny.Aws.Cryptography.MaterialProviders.Wrapped.Keys.Types._IError> result = _impl.SerializeKeyDescription(internalInput);
+ if (result.is_Failure) throw TypeConversion.FromDafny_CommonError(result.dtor_error);
+ return TypeConversion.FromDafny_N3_aws__N12_cryptography__N17_materialProviders__N7_wrapped__N4_keys__S29_SerializeKeyDescriptionOutput(result.dtor_value);
+}
+}
+}
