TestVectorsAwsCryptographicMaterialProviders/runtimes/net/Generated/KeyVectors/TestVectorKeyringInput.cs
@@ -1,0 +1,20 @@
+// Copyright Amazon.com Inc. or its affiliates. All Rights Reserved.
+// SPDX-License-Identifier: Apache-2.0
+// Do not modify this file. This file is machine generated, and any changes to it will be overwritten.
+using System;
+ using AWS.Cryptography.MaterialProviders.Wrapped.Keys; namespace AWS.Cryptography.MaterialProviders.Wrapped.Keys {
+ public class TestVectorKeyringInput {
+ private AWS.Cryptography.MaterialProviders.Wrapped.Keys.KeyDescription _keyDescription ;
+ public AWS.Cryptography.MaterialProviders.Wrapped.Keys.KeyDescription KeyDescription {
+ get { return this._keyDescription; }
+ set { this._keyDescription = value; }
+}
+ public bool IsSetKeyDescription () {
+ return this._keyDescription != null;
+}
+ public void Validate() {
+ if (!IsSetKeyDescription()) throw new System.ArgumentException("Missing value for required property 'KeyDescription'");
+
+}
+}
+}
