TestVectorsAwsCryptographicMaterialProviders/dafny/TestVectorsAwsCryptographicMaterialProviders/src/TestVectors.dfy
@@ -3,7 +3,7 @@
 
 include "LibraryIndex.dfy"
 include "CreateKeyrings.dfy"
-include "CreateKeyrings/CreateInvalidKeyrings.dfy"
+include "../../KeyVectors/src/Index.dfy"
 
 module {:options "-functionSyntax:4"} TestVectors {
   import Types = AwsCryptographyMaterialProvidersTypes
@@ -13,26 +13,20 @@ module {:options "-functionSyntax:4"} TestVectors {
   import opened StandardLibrary.UInt
   import UTF8
 
-  // Import all the keyring factorys
-  import CreateInvalidKeyrings
-  import CreateAwsKmsKeyrings
-  import CreateAwsKmsMultiKeyrings
-  import CreateAwsKmsMrkKeyrings
-  import CreateAwsKmsMrkMultiKeyrings
-  import CreateRawAesKeyrings
-  import CreateRawRsaKeyrings
+  import KeyVectors
+  import KeyVectorsTypes = AwsCryptographyMaterialProvidersWrappedKeysTypes
 
   datatype EncryptTest = EncryptTest(
-      input: Types.GetEncryptionMaterialsInput,
-      cmm: Types.ICryptographicMaterialsManager,
-      vector: EncryptTestVector
-    )
+    input: Types.GetEncryptionMaterialsInput,
+    cmm: Types.ICryptographicMaterialsManager,
+    vector: EncryptTestVector
+  )
 
   datatype DecryptTest = DecryptTest(
-      input: Types.DecryptMaterialsInput,
-      cmm: Types.ICryptographicMaterialsManager,
-      vector: DecryptTestVector
-    )
+    input: Types.DecryptMaterialsInput,
+    cmm: Types.ICryptographicMaterialsManager,
+    vector: DecryptTestVector
+  )
 
   method TestGetEncryptionMaterials(test: EncryptTest)
     returns (testResult: bool, edks: Option<Types.EncryptionMaterials>)
@@ -42,22 +36,22 @@ module {:options "-functionSyntax:4"} TestVectors {
     ensures testResult && test.vector.PositiveEncryptKeyringVector? ==> edks.Some?
   {
     print "\nTEST===> ",
-      test.vector.name,
-      if test.vector.description.Some? then "\n" + test.vector.description.value else "",
-      if test.vector.NegativeEncryptKeyringVector? then "\n" + test.vector.errorDescription else "", "\n";
+          test.vector.name,
+          if test.vector.description.Some? then "\n" + test.vector.description.value else "",
+          if test.vector.NegativeEncryptKeyringVector? then "\n" + test.vector.errorDescription else "", "\n";
 
     var result := test.cmm.GetEncryptionMaterials(test.input);
 
     testResult := match test.vector
-      case PositiveEncryptKeyringVector(_,_,_,_,_,_,_,_)
+      case PositiveEncryptKeyringVector(_,_,_,_,_,_,_,_,_)
         => result.Success?
       case NegativeEncryptKeyringVector(_,_,_,_,_,_,_,_,_)
         => !result.Success?;
 
     edks := if test.vector.PositiveEncryptKeyringVector? && result.Success? then
-        Some(result.value.encryptionMaterials)
-      else
-        None;
+      Some(result.value.encryptionMaterials)
+    else
+      None;
 
     if !testResult {
       print "FAILED! <-----------\n";
@@ -71,9 +65,9 @@ module {:options "-functionSyntax:4"} TestVectors {
     ensures test.cmm.ValidState()
   {
     print "\nTEST===> ",
-      test.vector.name,
-      if test.vector.description.Some? then "\n" + test.vector.description.value else "",
-      if test.vector.NegativeDecryptKeyringTest? then "\n" + test.vector.errorDescription else "\n";
+          test.vector.name,
+          if test.vector.description.Some? then "\n" + test.vector.description.value else "",
+          if test.vector.NegativeDecryptKeyringTest? then "\n" + test.vector.errorDescription else "\n";
 
     var result := test.cmm.DecryptMaterials(test.input);
 
@@ -89,18 +83,21 @@ module {:options "-functionSyntax:4"} TestVectors {
     }
   }
 
-  method ToEncryptTest(vector: EncryptTestVector)
+  method ToEncryptTest(keys: KeyVectors.KeyVectorsClient, vector: EncryptTestVector)
     returns (output: Result<EncryptTest, string>)
+    requires keys.ValidState()
+    modifies keys.Modifies
+    ensures keys.ValidState()
     ensures output.Success? ==>
-      && output.value.cmm.ValidState()
-      && fresh(output.value.cmm.Modifies)
+              && output.value.cmm.ValidState()
+              && fresh(output.value.cmm.Modifies)
   {
     var input := match vector
       case PositiveEncryptKeyringVector(
         _,_,
         encryptionContext, commitmentPolicy, algorithmSuite, maxPlaintextLength, requiredEncryptionContextKeys,
-        _
-      ) =>
+        _,_
+        ) =>
         Types.GetEncryptionMaterialsInput(
           encryptionContext := encryptionContext,
           commitmentPolicy := commitmentPolicy,
@@ -112,7 +109,7 @@ module {:options "-functionSyntax:4"} TestVectors {
         _,_,
         encryptionContext, commitmentPolicy, algorithmSuite, maxPlaintextLength, requiredEncryptionContextKeys,
         _, _
-      ) =>
+        ) =>
         Types.GetEncryptionMaterialsInput(
           encryptionContext := encryptionContext,
           commitmentPolicy := commitmentPolicy,
@@ -123,31 +120,37 @@ module {:options "-functionSyntax:4"} TestVectors {
 
     var mpl :- expect WrappedMaterialProviders.WrappedMaterialProviders();
 
-    var keyring :- ToKeyring(if vector.PositiveEncryptKeyringVector? then
-        vector.keyringInfos.encryptInfo
-      else
-        vector.keyringInfo);
+    var maybeKeyring := keys.CreateWappedTestVectorKeyring(
+      KeyVectorsTypes.TestVectorKeyringInput(
+        keyDescription := if vector.PositiveEncryptKeyringVector? then
+          vector.encryptDescription
+        else
+          vector.keyDescription
+      ));
+    var keyring :- maybeKeyring.MapFailure(e => "Keyring failure");
 
     var maybeCmm := mpl
-      .CreateDefaultCryptographicMaterialsManager(
-        Types.CreateDefaultCryptographicMaterialsManagerInput( keyring := keyring )
-      );
+    .CreateDefaultCryptographicMaterialsManager(
+      Types.CreateDefaultCryptographicMaterialsManagerInput( keyring := keyring )
+    );
     var cmm :- maybeCmm.MapFailure(e => "CMM failure");
 
     return Success(EncryptTest(
-      input := input,
-      cmm := cmm,
-      vector := vector
-    ));
-
+                     input := input,
+                     cmm := cmm,
+                     vector := vector
+                   ));
   }
 
-  method ToDecryptTest(test: EncryptTest, materials: Types.EncryptionMaterials)
+  method ToDecryptTest(keys: KeyVectors.KeyVectorsClient, test: EncryptTest, materials: Types.EncryptionMaterials)
     returns (output: Result<DecryptTest, string>)
     requires test.vector.PositiveEncryptKeyringVector?
+    requires keys.ValidState()
+    modifies keys.Modifies
+    ensures keys.ValidState()
     ensures output.Success? ==>
-      && output.value.cmm.ValidState()
-      && fresh(output.value.cmm.Modifies)
+              && output.value.cmm.ValidState()
+              && fresh(output.value.cmm.Modifies)
   {
 
     // TODO remove requiredEncryptionContextKeys, and add to reproducedEncryptionContext
@@ -166,7 +169,7 @@ module {:options "-functionSyntax:4"} TestVectors {
       commitmentPolicy := test.vector.commitmentPolicy,
       encryptedDataKeys := materials.encryptedDataKeys,
       encryptionContext := materials.encryptionContext,
-      keyrings := test.vector.keyringInfos.decryptInfo,
+      keyDescription := test.vector.decryptDescription,
       description := if test.vector.description.Some? then
         Some("Decryption for " + test.vector.description.value)
       else None,
@@ -175,326 +178,79 @@ module {:options "-functionSyntax:4"} TestVectors {
 
     var mpl :- expect WrappedMaterialProviders.WrappedMaterialProviders();
 
-    var keyring :- ToKeyring(test.vector.keyringInfos.decryptInfo);
+    var maybeKeyring := keys.CreateWappedTestVectorKeyring(
+      KeyVectorsTypes.TestVectorKeyringInput(
+        keyDescription := vector.keyDescription
+      )
+    );
+    var keyring :- maybeKeyring.MapFailure(e => "Keyring failure");
 
     var maybeCmm := mpl
-      .CreateDefaultCryptographicMaterialsManager(
-        Types.CreateDefaultCryptographicMaterialsManagerInput( keyring := keyring )
-      );
+    .CreateDefaultCryptographicMaterialsManager(
+      Types.CreateDefaultCryptographicMaterialsManagerInput( keyring := keyring )
+    );
     var cmm :- maybeCmm.MapFailure(e => "CMM failure");
 
     return Success(DecryptTest(
-      input := input,
-      cmm := cmm,
-      vector := vector
-    ));
-  }
-
-  method ToKeyring(info: KeyringInfo)
-    returns (output: Result<Types.IKeyring, string>)
-    ensures output.Success? ==>
-      && output.value.ValidState()
-      && fresh(output.value.Modifies)
-  {
-    var mpl :- expect WrappedMaterialProviders.WrappedMaterialProviders();
-    var KeyringInfo(description, material) := info;
-    match (description, material)
-      case (
-        InvalidKeyring(key),
-        Some(InvalidMaterial(
-          _,
-          algorithmSuite,
-          encryptionContext,
-          encryptedDataKeys,
-          requiredEncryptionContextKeys,
-          plaintextDataKey,
-          signingKey,
-          verificationKey,
-          symmetricSigningKeys
-        ))
-      ) => {
-
-        var encrypt := Types.EncryptionMaterials(
-          algorithmSuite := algorithmSuite,
-          encryptedDataKeys := encryptedDataKeys,
-          encryptionContext := encryptionContext,
-          requiredEncryptionContextKeys := requiredEncryptionContextKeys,
-          plaintextDataKey := plaintextDataKey,
-          signingKey := signingKey,
-          symmetricSigningKeys := symmetricSigningKeys
-        );
-        var decrypt := Types.DecryptionMaterials(
-          algorithmSuite := algorithmSuite,
-          encryptionContext := encryptionContext,
-          requiredEncryptionContextKeys := requiredEncryptionContextKeys,
-          plaintextDataKey := plaintextDataKey,
-          verificationKey := verificationKey,
-          symmetricSigningKey := None // need to pass one vs many :(
-        );
-
-        var keyring := CreateInvalidKeyrings.CreateInvalidMaterialKeyring(encrypt, decrypt);
-        return Success(keyring);
-      }
-
-      case (KMSInfo(key), Some(KMS(_, _, _, keyIdentifier))) => {
-        var input := Types.CreateAwsKmsMultiKeyringInput(
-          generator := Some(keyIdentifier),
-          kmsKeyIds := None,
-          clientSupplier := None,
-          grantTokens := None
-        );
-        var keyring := mpl.CreateAwsKmsMultiKeyring(input);
-        return keyring.MapFailure(e => "Unable to CreateAwsKmsMultiKeyring");
-      }
-      case (KmsMrkAware(key), Some(KMS(_, _, _, keyIdentifier))) => {
-        var input := Types.CreateAwsKmsMrkMultiKeyringInput(
-          generator := Some(keyIdentifier),
-          kmsKeyIds := None,
-          clientSupplier := None,
-          grantTokens := None
-        );
-        var keyring := mpl.CreateAwsKmsMrkMultiKeyring(input);
-        return keyring.MapFailure(e => "Unable to CreateAwsKmsMrkMultiKeyring");
-      }
-      case (
-        KmsMrkAwareDiscovery(defaultMrkRegion, awsKmsDiscoveryFilter),
-        Some(KMS(_, _, decrypt, keyIdentifier))
-      ) => {
-        :- Need(decrypt, "Discovery only supports decrypt.");
-        var input := Types.CreateAwsKmsDiscoveryMultiKeyringInput(
-          regions := [defaultMrkRegion],
-          discoveryFilter := awsKmsDiscoveryFilter,
-          clientSupplier := None,
-          grantTokens := None
-        );
-        var keyring := mpl.CreateAwsKmsDiscoveryMultiKeyring(input);
-        return keyring.MapFailure(e => "Unable to CreateAwsKmsDiscoveryMultiKeyring");
-      }
-      case (
-        RawAES(key, providerId),
-        Some(Symetric(_, _, _, algorithm, bits, encoding, wrappingKey, keyIdentifier))
-      ) => {
-        var wrappingAlg :- match bits
-          case 128 => Success(Types.ALG_AES128_GCM_IV12_TAG16)
-          case 192 => Success(Types.ALG_AES192_GCM_IV12_TAG16)
-          case 256 => Success(Types.ALG_AES256_GCM_IV12_TAG16)
-          case _ => Failure("Not a supported bit length");
-
-        var input := Types.CreateRawAesKeyringInput(
-          keyNamespace := providerId,
-          keyName := keyIdentifier,
-          wrappingKey := wrappingKey,
-          wrappingAlg := wrappingAlg
-        );
-        var keyring := mpl.CreateRawAesKeyring(input);
-        return keyring.MapFailure(e => "Unable to CreateRawAesKeyring");
-      }
-      case (
-        RawRSA(key, providerId, padding),
-        Some(PrivateRSA(_, _, decrypt, algorithm, bits, encoding, material, keyIdentifier))
-      ) => {
-        :- Need(decrypt, "Private RSA keys only supports decrypt.");
-        var privateKeyPemBytes :- UTF8.Encode(material);
-        var input := Types.CreateRawRsaKeyringInput(
-          keyNamespace := providerId,
-          keyName := keyIdentifier,
-          paddingScheme := padding,
-          publicKey := None,
-          privateKey := Some(privateKeyPemBytes)
-        );
-        var keyring := mpl.CreateRawRsaKeyring(input);
-        return keyring.MapFailure(e => "Unable to CreateRawRsaKeyring");
-      }
-      case (
-        RawRSA(key, providerId, padding),
-        Some(PublicRSA(_, encrypt, _, algorithm, bits, encoding, material, keyIdentifier))
-      ) => {
-        :- Need(encrypt, "Public RSA keys only supports encrypt.");
-        var publicKeyPemBytes :- UTF8.Encode(material);
-        var input := Types.CreateRawRsaKeyringInput(
-          keyNamespace := providerId,
-          keyName := keyIdentifier,
-          paddingScheme := padding,
-          publicKey := Some(publicKeyPemBytes),
-          privateKey := None
-        );
-        var keyring := mpl.CreateRawRsaKeyring(input);
-        return keyring.MapFailure(e => "Unable to CreateRawRsaKeyring");
-      }
-
-      case _ => {
-        return Failure("Unsuported Material combination");
-      }
+                     input := input,
+                     cmm := cmm,
+                     vector := vector
+                   ));
   }
 
   datatype EncryptTestVector =
     | PositiveEncryptKeyringVector(
-      name: string,
-      description: Option<string>,
-      encryptionContext: Types.EncryptionContext,
-      commitmentPolicy: Types.CommitmentPolicy,
-      // algorithmSuiteId is NOT an option
-      // because test vectors are not the place to test defaults
-      algorithmSuite: Types.AlgorithmSuiteInfo,
-      maxPlaintextLength: Option<UInt.int64>,
-      requiredEncryptionContextKeys: Option<Types.EncryptionContextKeys>,
-      keyringInfos: PositiveKeyringInfo
-    )
+        name: string,
+        description: Option<string>,
+        encryptionContext: Types.EncryptionContext,
+        commitmentPolicy: Types.CommitmentPolicy,
+        // algorithmSuiteId is NOT an option
+        // because test vectors are not the place to test defaults
+        algorithmSuite: Types.AlgorithmSuiteInfo,
+        maxPlaintextLength: Option<UInt.int64>,
+        requiredEncryptionContextKeys: Option<Types.EncryptionContextKeys>,
+        encryptDescription: KeyVectorsTypes.KeyDescription,
+        decryptDescription: KeyVectorsTypes.KeyDescription
+      )
     | NegativeEncryptKeyringVector(
-      name: string,
-      description: Option<string>,
-      encryptionContext: Types.EncryptionContext,
-      commitmentPolicy: Types.CommitmentPolicy,
-      // algorithmSuiteId is NOT an option
-      // because test vectors are not the place to test defaults
-      algorithmSuite: Types.AlgorithmSuiteInfo,
-      maxPlaintextLength: Option<UInt.int64>,
-      requiredEncryptionContextKeys: Option<Types.EncryptionContextKeys>,
-      errorDescription: string,
-      keyringInfo: KeyringInfo
-    )
-    // | PositiveEncryptCMMTest
-    // | NegativeEncryptCMMTest
-
-  datatype PositiveKeyringInfo = PositiveKeyringInfo(
-    encryptInfo: KeyringInfo,
-    decryptInfo: KeyringInfo
-  )
+        name: string,
+        description: Option<string>,
+        encryptionContext: Types.EncryptionContext,
+        commitmentPolicy: Types.CommitmentPolicy,
+        // algorithmSuiteId is NOT an option
+        // because test vectors are not the place to test defaults
+        algorithmSuite: Types.AlgorithmSuiteInfo,
+        maxPlaintextLength: Option<UInt.int64>,
+        requiredEncryptionContextKeys: Option<Types.EncryptionContextKeys>,
+        errorDescription: string,
+        keyDescription: KeyVectorsTypes.KeyDescription
+      )
+      // | PositiveEncryptCMMTest
+      // | NegativeEncryptCMMTest
 
   datatype DecryptTestVector =
     | PositiveDecryptKeyringTest(
-      name: string,
-      algorithmSuite: Types.AlgorithmSuiteInfo,
-      commitmentPolicy: Types.CommitmentPolicy,
-      encryptedDataKeys: Types.EncryptedDataKeyList,
-      encryptionContext: Types.EncryptionContext,
-      keyrings: KeyringInfo,
-      description: Option<string> := None,
-      reproducedEncryptionContext: Option<Types.EncryptionContext> := None
-    )
+        name: string,
+        algorithmSuite: Types.AlgorithmSuiteInfo,
+        commitmentPolicy: Types.CommitmentPolicy,
+        encryptedDataKeys: Types.EncryptedDataKeyList,
+        encryptionContext: Types.EncryptionContext,
+        keyDescription: KeyVectorsTypes.KeyDescription,
+        description: Option<string> := None,
+        reproducedEncryptionContext: Option<Types.EncryptionContext> := None
+      )
     | NegativeDecryptKeyringTest(
-      name: string,
-      algorithmSuite: Types.AlgorithmSuiteInfo,
-      commitmentPolicy: Types.CommitmentPolicy,
-      encryptedDataKeys: Types.EncryptedDataKeyList,
-      encryptionContext: Types.EncryptionContext,
-      errorDescription: string,
-      keyrings: KeyringInfo,
-      reproducedEncryptionContext: Option<Types.EncryptionContext> := None,
-      description: Option<string> := None
-    )
-    // | PositiveDecryptCMMTest
-    // | NegativeDecryptCMMTest
-
-
-
-
-  datatype KeyDescription =
-    | KMSInfo(key: string)
-    | KmsMrkAware(key: string)
-    | KmsMrkAwareDiscovery(
-      defaultMrkRegion: string,
-      awsKmsDiscoveryFilter: Option<Types.DiscoveryFilter> := None
-    )
-    | RawRSA( key: string, providerId: string, padding: Types.PaddingScheme)
-    | RawAES( key: string, providerId: string )
-    | InvalidKeyring( key: string)
-
-  datatype KeyMaterial =
-    | Symetric(
-      name: string,
-      encrypt: bool, decrypt: bool,
-      algorithm: string,
-      bits: nat,
-      encoding: string,
-      wrappingKey: Types.Secret,
-      keyIdentifier: string
-    )
-    | PrivateRSA(
-      name: string,
-      encrypt: bool, decrypt: bool,
-      algorithm: string,
-      bits: nat,
-      encoding: string,
-      material: string,
-      keyIdentifier: string
-    )
-    | PublicRSA(
-      name: string,
-      encrypt: bool, decrypt: bool,
-      bits: nat,
-      algorithm: string,
-      encoding: string,
-      material: string,
-      keyIdentifier: string
-    )
-    | KMS(
-      name: string,
-      encrypt: bool, decrypt: bool,
-      keyIdentifier: string
-    )
-    | InvalidMaterial(
-      name: string,
-      algorithmSuite: Types.AlgorithmSuiteInfo,
-      encryptionContext: Types.EncryptionContext,
-      encryptedDataKeys: Types.EncryptedDataKeyList,
-      requiredEncryptionContextKeys: Types.EncryptionContextKeys,
-      plaintextDataKey: Option<Types.Secret> := None,
-      signingKey: Option<Types.Secret> := None,
-      verificationKey: Option<Types.Secret> := None,
-      symmetricSigningKeys: Option<Types.SymmetricSigningKeyList> := None
-    )
-
-  datatype KeyringInfo = KeyringInfo(
-    description: KeyDescription,
-    material: Option<KeyMaterial>
-  )
-
-  type KeyMaterialString = s: string | KeyMaterialString?(s) witness *
-  predicate KeyMaterialString?(s: string)
-  {
-    || s == "invalid"
-    || s == "aws-kms"
-    || s == "symmetric"
-    || s == "private"
-    || s == "public"
-  }
-
-  type KeyDescriptionString = s: string | KeyDescriptionString?(s) witness *
-  predicate KeyDescriptionString?(s: string)
-  {
-    || s == "invalid"
-    || s == "aws-kms"
-    || s == "aws-kms-mrk-aware"
-    || s == "aws-kms-mrk-aware-discovery"
-    || s == "raw"
-  }
-
-  type RawAlgorithmString = s: string | RawAlgorithmString?(s) witness *
-  predicate RawAlgorithmString?(s: string)
-  {
-    || s == "aes"
-    || s == "rsa"
-  }
-
-  type PaddingAlgorithmString = s: string | PaddingAlgorithmString?(s) witness *
-  predicate PaddingAlgorithmString?(s: string)
-  {
-    || s == "pkcs1"
-    || s == "oaep-mgf1"
-  }
-
-  type PaddingHashString = s: string | PaddingHashString?(s) witness *
-  predicate PaddingHashString?(s: string)
-  {
-    || s == "sha1"
-    || s == "sha1"
-    || s == "sha256"
-    || s == "sha384"
-    || s == "sha512"
-  }
-
-
-
+        name: string,
+        algorithmSuite: Types.AlgorithmSuiteInfo,
+        commitmentPolicy: Types.CommitmentPolicy,
+        encryptedDataKeys: Types.EncryptedDataKeyList,
+        encryptionContext: Types.EncryptionContext,
+        errorDescription: string,
+        keyDescription: KeyVectorsTypes.KeyDescription,
+        reproducedEncryptionContext: Option<Types.EncryptionContext> := None,
+        description: Option<string> := None
+      )
+      // | PositiveDecryptCMMTest
+      // | NegativeDecryptCMMTest
 
 }
