TestVectorsAwsCryptographicMaterialProviders/dafny/KeyVectors/src/KeyDescription.dfy
@@ -1,0 +1,114 @@
+// Copyright Amazon.com Inc. or its affiliates. All Rights Reserved.
+// SPDX-License-Identifier: Apache-2.0
+
+include "../Model/AwsCryptographyMaterialProvidersWrappedKeysTypes.dfy"
+  // Yes, this is reaching across.
+  // idealy all these functions would exist in the STD Library.
+include "../../TestVectorsAwsCryptographicMaterialProviders/src/JSONHelpers.dfy"
+
+module {:options "-functionSyntax:4"} KeyDescription {
+  import opened Wrappers
+  import opened JSON.AST
+  import AwsCryptographyMaterialProvidersTypes
+  import opened Types = AwsCryptographyMaterialProvidersWrappedKeysTypes
+  import opened JSONHelpers
+
+  function ToKeyDescription(obj: JSON): Result<KeyDescription, string>
+  {
+    :- Need(obj.Object?, "KeyDescription not an object");
+    var obj := obj.obj;
+    var typString := "type";
+    var typ :- GetString(typString, obj);
+
+    :- Need(KeyDescriptionString?(typ), "Unsupported KeyDescription type:" + typ);
+    var key :- GetString("key", obj);
+
+    match typ
+    case "invalid" =>
+      Success(Invalid(InvalidKeyring( keyId := key )))
+    case "aws-kms" =>
+      Success(Kms(KMSInfo( keyId := key )))
+    case "aws-kms-mrk-aware" =>
+      Success(KmsMrk(KmsMrkAware( keyId := key )))
+    case "aws-kms-mrk-aware-discovery" =>
+      var defaultMrkRegion :- GetString("partition", obj);
+      var filter := GetObject("aws-kms-discovery-filter", obj);
+      var awsKmsDiscoveryFilter := ToDiscoveryFilter(obj);
+      Success(KmsMrkDiscovery(KmsMrkAwareDiscovery(
+                                keyId := "aws-kms-mrk-aware-discovery",
+                                defaultMrkRegion := defaultMrkRegion,
+                                awsKmsDiscoveryFilter := awsKmsDiscoveryFilter
+                              )))
+    case "raw" =>
+      var algorithm :- GetString("encryption-algorithm", obj);
+      var providerId :- GetString("provider-id", obj);
+      :- Need(RawAlgorithmString?(algorithm), "Unsupported algorithm:" + algorithm);
+      match algorithm
+      case "aes" =>
+        Success(AES(RawAES( keyId := key, providerId := providerId )))
+      case "rsa" =>
+        var paddingAlgorithm :- GetString("padding-algorithm", obj);
+        var paddingHash :- GetString("padding-hash", obj);
+        :- Need(PaddingAlgorithmString?(paddingAlgorithm), "Unsupported paddingAlgorithm:" + paddingAlgorithm);
+        :- Need(PaddingHashString?(paddingHash), "Unsupported paddingHash:" + paddingHash);
+
+        match paddingAlgorithm
+        case "pkcs1" =>
+          :- Need(paddingHash == "sha1", "Unsupported padding with pkcs1:" + paddingHash);
+          Success(RSA(RawRSA( keyId := key, providerId := providerId, padding := AwsCryptographyMaterialProvidersTypes.PKCS1 )))
+        case "oaep-mgf1" => match paddingHash
+          case "sha1" => Success(RSA(RawRSA( keyId := key, providerId := providerId, padding := AwsCryptographyMaterialProvidersTypes.OAEP_SHA1_MGF1 )))
+          case "sha256" => Success(RSA(RawRSA( keyId := key, providerId := providerId, padding := AwsCryptographyMaterialProvidersTypes.OAEP_SHA256_MGF1 )))
+          case "sha384" => Success(RSA(RawRSA( keyId := key, providerId := providerId, padding := AwsCryptographyMaterialProvidersTypes.OAEP_SHA384_MGF1 )))
+          case "sha512" => Success(RSA(RawRSA( keyId := key, providerId := providerId, padding := AwsCryptographyMaterialProvidersTypes.OAEP_SHA512_MGF1 )))
+  }
+
+  function ToDiscoveryFilter(obj: seq<(string, JSON)>)
+    : Option<AwsCryptographyMaterialProvidersTypes.DiscoveryFilter>
+  {
+    var filter :- GetObject("aws-kms-discovery-filter", obj).ToOption();
+    var partition :- GetString("partition", filter).ToOption();
+    var accountIds :- GetArrayString("account-ids", filter).ToOption();
+    Some(AwsCryptographyMaterialProvidersTypes.DiscoveryFilter(
+           partition := partition,
+           accountIds := accountIds
+         ))
+  }
+
+
+
+  type KeyDescriptionString = s: string | KeyDescriptionString?(s) witness *
+  predicate KeyDescriptionString?(s: string)
+  {
+    || s == "invalid"
+    || s == "aws-kms"
+    || s == "aws-kms-mrk-aware"
+    || s == "aws-kms-mrk-aware-discovery"
+    || s == "raw"
+  }
+
+  type RawAlgorithmString = s: string | RawAlgorithmString?(s) witness *
+  predicate RawAlgorithmString?(s: string)
+  {
+    || s == "aes"
+    || s == "rsa"
+  }
+
+  type PaddingAlgorithmString = s: string | PaddingAlgorithmString?(s) witness *
+  predicate PaddingAlgorithmString?(s: string)
+  {
+    || s == "pkcs1"
+    || s == "oaep-mgf1"
+  }
+
+  type PaddingHashString = s: string | PaddingHashString?(s) witness *
+  predicate PaddingHashString?(s: string)
+  {
+    || s == "sha1"
+    || s == "sha1"
+    || s == "sha256"
+    || s == "sha384"
+    || s == "sha512"
+  }
+
+}
