TestVectorsAwsCryptographicMaterialProviders/dafny/KeyVectors/src/KeyringFromKeyDescription.dfy
@@ -1,0 +1,161 @@
+// Copyright Amazon.com Inc. or its affiliates. All Rights Reserved.
+// SPDX-License-Identifier: Apache-2.0
+
+include "../Model/AwsCryptographyMaterialProvidersWrappedKeysTypes.dfy"
+  // Yes this is including from somewhere else.
+include "../../TestVectorsAwsCryptographicMaterialProviders/src/LibraryIndex.dfy"
+include "KeyMaterial.dfy"
+include "CreateInvalidKeyrings.dfy"
+
+module {:options "-functionSyntax:4"} KeyringFromKeyDescription {
+  import opened Types = AwsCryptographyMaterialProvidersWrappedKeysTypes
+  import MPL = AwsCryptographyMaterialProvidersTypes
+    // import WrappedMaterialProviders
+  import opened Wrappers
+  import KeyMaterial
+  import CreateInvalidKeyrings
+
+  datatype KeyringInfo = KeyringInfo(
+    description: KeyDescription,
+    material: Option<KeyMaterial.KeyMaterial>
+  )
+
+  method ToKeyring(mpl: MPL.IAwsCryptographicMaterialProvidersClient, info: KeyringInfo)
+    returns (output: Result<MPL.IKeyring, Error>)
+    requires mpl.ValidState()
+    modifies mpl.Modifies
+    ensures mpl.ValidState()
+    ensures output.Success? ==>
+              && output.value.ValidState()
+              && fresh(output.value.Modifies - mpl.Modifies - {mpl.History})
+  {
+    var KeyringInfo(description, material) := info;
+    match (description, material)
+    case (
+      Invalid(InvalidKeyring(key)),
+        Some(InvalidMaterial(
+        _,
+        algorithmSuite,
+        encryptionContext,
+        encryptedDataKeys,
+        requiredEncryptionContextKeys,
+        plaintextDataKey,
+        signingKey,
+        verificationKey,
+        symmetricSigningKeys
+        ))
+        ) => {
+
+      var encrypt := MPL.EncryptionMaterials(
+        algorithmSuite := algorithmSuite,
+        encryptedDataKeys := encryptedDataKeys,
+        encryptionContext := encryptionContext,
+        requiredEncryptionContextKeys := requiredEncryptionContextKeys,
+        plaintextDataKey := plaintextDataKey,
+        signingKey := signingKey,
+        symmetricSigningKeys := symmetricSigningKeys
+      );
+      var decrypt := MPL.DecryptionMaterials(
+        algorithmSuite := algorithmSuite,
+        encryptionContext := encryptionContext,
+        requiredEncryptionContextKeys := requiredEncryptionContextKeys,
+        plaintextDataKey := plaintextDataKey,
+        verificationKey := verificationKey,
+        symmetricSigningKey := None // need to pass one vs many :(
+      );
+
+      var keyring := CreateInvalidKeyrings.CreateInvalidMaterialKeyring(encrypt, decrypt);
+      return Success(keyring);
+    }
+
+    case (Kms(KMSInfo(key)), Some(KMS(_, _, _, keyIdentifier))) => {
+      var input := MPL.CreateAwsKmsMultiKeyringInput(
+        generator := Some(keyIdentifier),
+        kmsKeyIds := None,
+        clientSupplier := None,
+        grantTokens := None
+      );
+      var keyring := mpl.CreateAwsKmsMultiKeyring(input);
+      return keyring.MapFailure(e => AwsCryptographyMaterialProviders(e));
+    }
+    case (KmsMrk(KmsMrkAware(key)), Some(KMS(_, _, _, keyIdentifier))) => {
+      var input := MPL.CreateAwsKmsMrkMultiKeyringInput(
+        generator := Some(keyIdentifier),
+        kmsKeyIds := None,
+        clientSupplier := None,
+        grantTokens := None
+      );
+      var keyring := mpl.CreateAwsKmsMrkMultiKeyring(input);
+      return keyring.MapFailure(e => AwsCryptographyMaterialProviders(e));
+    }
+    case (
+      KmsMrkDiscovery(KmsMrkAwareDiscovery(_, defaultMrkRegion, awsKmsDiscoveryFilter)),
+        Some(KMS(_, _, decrypt, keyIdentifier))
+        ) => {
+      :- Need(decrypt, KeyVectorException( message := "Discovery only supports decrypt."));
+      var input := MPL.CreateAwsKmsDiscoveryMultiKeyringInput(
+        regions := [defaultMrkRegion],
+        discoveryFilter := awsKmsDiscoveryFilter,
+        clientSupplier := None,
+        grantTokens := None
+      );
+      var keyring := mpl.CreateAwsKmsDiscoveryMultiKeyring(input);
+      return keyring.MapFailure(e => AwsCryptographyMaterialProviders(e));
+    }
+    case (
+      AES(RawAES(key, providerId)),
+        Some(Symetric(_, _, _, algorithm, bits, encoding, wrappingKey, keyIdentifier))
+        ) => {
+      var wrappingAlg :- match bits
+        case 128 => Success(MPL.ALG_AES128_GCM_IV12_TAG16)
+        case 192 => Success(MPL.ALG_AES192_GCM_IV12_TAG16)
+        case 256 => Success(MPL.ALG_AES256_GCM_IV12_TAG16)
+        case _ => Failure(KeyVectorException( message := "Not a supported bit length" ));
+
+      var input := MPL.CreateRawAesKeyringInput(
+        keyNamespace := providerId,
+        keyName := keyIdentifier,
+        wrappingKey := wrappingKey,
+        wrappingAlg := wrappingAlg
+      );
+      var keyring := mpl.CreateRawAesKeyring(input);
+      return keyring.MapFailure(e => AwsCryptographyMaterialProviders(e));
+    }
+    case (
+      RSA(RawRSA(key, providerId, padding)),
+        Some(PrivateRSA(_, _, decrypt, algorithm, bits, encoding, material, keyIdentifier))
+        ) => {
+      :- Need(decrypt, KeyVectorException( message := "Private RSA keys only supports decrypt." ));
+      var privateKeyPemBytes :- UTF8.Encode(material).MapFailure(e => KeyVectorException( message := e ));
+      var input := MPL.CreateRawRsaKeyringInput(
+        keyNamespace := providerId,
+        keyName := keyIdentifier,
+        paddingScheme := padding,
+        publicKey := None,
+        privateKey := Some(privateKeyPemBytes)
+      );
+      var keyring := mpl.CreateRawRsaKeyring(input);
+      return keyring.MapFailure(e => AwsCryptographyMaterialProviders(e));
+    }
+    case (
+      RSA(RawRSA(key, providerId, padding)),
+        Some(PublicRSA(_, encrypt, _, algorithm, bits, encoding, material, keyIdentifier))
+        ) => {
+      :- Need(encrypt, KeyVectorException( message := "Public RSA keys only supports encrypt." ));
+      var publicKeyPemBytes :- UTF8.Encode(material).MapFailure(e => KeyVectorException( message := e ));
+      var input := MPL.CreateRawRsaKeyringInput(
+        keyNamespace := providerId,
+        keyName := keyIdentifier,
+        paddingScheme := padding,
+        publicKey := Some(publicKeyPemBytes),
+        privateKey := None
+      );
+      var keyring := mpl.CreateRawRsaKeyring(input);
+      return keyring.MapFailure(e => AwsCryptographyMaterialProviders(e));
+    }
+
+    case _ => {
+      return Failure(KeyVectorException( message := "Unsuported Material combination"));
+    }
+  }
+}
