TestVectorsAwsCryptographicMaterialProviders/dafny/TestVectorsAwsCryptographicMaterialProviders/src/Index.dfy
@@ -34,7 +34,7 @@ module WrappedMaterialProvidersMain {
 
   method EncryptTestVectors() {
 
-    
+
 
   }
 
