TestVectorsAwsCryptographicMaterialProviders/dafny/TestVectorsAwsCryptographicMaterialProviders/src/ParseJsonManifests.dfy
@@ -17,131 +17,19 @@ module {:options "-functionSyntax:4"} ParseJsonManifests {
   import UTF8
   import Seq
   import opened StandardLibrary.UInt
+  import BoundedInts
   import opened JSONHelpers
   import opened TestVectors
   import HexStrings
   import Base64
   import CompleteVectors
-  // This is a HACK!
-  // This is *ONLY* because this is wrapping the MPL
+  import KeyVectors
+  import KeyVectorsTypes = AwsCryptographyMaterialProvidersWrappedKeysTypes
+    // This is a HACK!
+    // This is *ONLY* because this is wrapping the MPL
   import AlgorithmSuites
 
-  function BuildKeyMaterials(obj: seq<(string, JSON)>): Result<map<string, KeyMaterial>, string>
-  {
-    if |obj| == 0 then
-      Success(map[])
-    else
-      var name := obj[0].0;
-      var keyMaterial :- ToKeyMaterial(name, obj[0].1);
-      var tail :- BuildKeyMaterials(obj[1..]);
-      Success(map[ name := keyMaterial] + tail)
-  }
-
-  function ToKeyMaterial(name: string, obj: JSON): Result<KeyMaterial, string>
-  {
-    :- Need(obj.Object?, "KeyDescription not an object");
-    var obj := obj.obj;
-    var typString := "type";
-    var typ :- GetString(typString, obj);
-
-    :- Need(TestVectors.KeyMaterialString?(typ), "Unsupported KeyMaterial type:" + typ);
-
-    match typ
-      case "invalid" =>
-        var algorithmSuiteHex :- GetString("algorithmSuiteId", obj);
-        :- Need(HexStrings.IsLooseHexString(algorithmSuiteHex), "Not hex encoded binnary");
-        var binaryId := HexStrings.FromHexString(algorithmSuiteHex);
-        var algorithmSuite :- AlgorithmSuites
-          .GetAlgorithmSuiteInfo(binaryId)
-          .MapFailure(e => "Invalid Suite:" + algorithmSuiteHex);
-
-        var encryptionContextStrings :- SmallObjectToStringStringMap("encryptionContext", obj);
-        var encryptionContext :- utf8EncodeMap(encryptionContextStrings);
-
-        var keysAsStrings :- GetArrayString("requiredEncryptionContextKeys", obj);
-        var requiredEncryptionContextKeys :- utf8EncodeSeq(keysAsStrings);
-
-        var encryptedDataKeysJSON :- GetArrayObject("encryptedDataKeys", obj);
-        var encryptedDataKeys :- Seq.MapWithResult(ToEncryptedDataKey, encryptedDataKeysJSON);
-
-        var plaintextDataKeyEncoded :- GetOptionalString("plaintextDataKey", obj);
-        var plaintextDataKey :- if plaintextDataKeyEncoded.Some? then
-            var result := Base64.Decode(plaintextDataKeyEncoded.value);
-            if result.Success? then Success(Some(result.value)) else Failure(result.error)
-          else Success(None);
-        var signingKey :- GetOptionalString("signingKey", obj);
-        var verificationKey :- GetOptionalString("verificationKey", obj);
-        var symmetricSigningKeys := GetArrayString("symmetricSigningKeys", obj).ToOption();
-
-        Success(InvalidMaterial(
-          name := name,
-          algorithmSuite := algorithmSuite,
-          encryptionContext := encryptionContext,
-          encryptedDataKeys := encryptedDataKeys,
-          requiredEncryptionContextKeys := requiredEncryptionContextKeys,
-          plaintextDataKey := plaintextDataKey,
-          // This is just for now...
-          signingKey := None,
-          verificationKey := None,
-          symmetricSigningKeys := None
-        ))
-      case _ =>
-        var encrypt :- GetBool("encrypt", obj);
-        var decrypt :- GetBool("decrypt", obj);
-        var keyIdentifier :- GetString("key-id", obj);
-        
-        match typ
-          case "aws-kms" =>
-            Success(KeyMaterial.KMS(
-              name := name,
-              encrypt := encrypt,
-              decrypt := decrypt,
-              keyIdentifier := keyIdentifier
-            ))
-          case _ =>
-            var algorithm :- GetString("algorithm", obj);
-            var bits :- GetNat("bits", obj);
-            var encoding :- GetString("encoding", obj);
-            var material :- GetString("material", obj);
-
-            match typ
-              case "symmetric" =>
-                var materialBytes :- Base64.Decode(material);
-                Success(Symetric(
-                  name := name,
-                  encrypt := encrypt,
-                  decrypt := decrypt,
-                  keyIdentifier := keyIdentifier,
-                  algorithm := algorithm,
-                  bits := bits,
-                  encoding := encoding,
-                  wrappingKey := materialBytes
-                ))
-              case "private" =>
-                Success(PrivateRSA(
-                  name := name,
-                  encrypt := encrypt,
-                  decrypt := decrypt,
-                  keyIdentifier := keyIdentifier,
-                  algorithm := algorithm,
-                  bits := bits,
-                  encoding := encoding,
-                  material := material
-                ))
-              case "public" =>
-                Success(PublicRSA(
-                  name := name,
-                  encrypt := encrypt,
-                  decrypt := decrypt,
-                  keyIdentifier := keyIdentifier,
-                  algorithm := algorithm,
-                  bits := bits,
-                  encoding := encoding,
-                  material := material
-                ))
-  }
-
-  function BuildEncryptTestVector(keys: map<string, KeyMaterial>, obj: seq<(string, JSON)>)
+  function BuildEncryptTestVector(keys: KeyVectors.KeyVectorsClient, obj: seq<(string, JSON)>)
     : Result<seq<EncryptTestVector>, string>
   {
     if |obj| == 0 then
@@ -153,7 +41,7 @@ module {:options "-functionSyntax:4"} ParseJsonManifests {
       Success([ encryptVector ] + tail)
   }
 
-  function ToEncryptTestVector(keys: map<string, KeyMaterial>, name: string, obj: JSON)
+  function ToEncryptTestVector(keys: KeyVectors.KeyVectorsClient, name: string, obj: JSON)
     : Result<EncryptTestVector, string>
   {
     :- Need(obj.Object?, "EncryptTestVector not an object");
@@ -171,178 +59,70 @@ module {:options "-functionSyntax:4"} ParseJsonManifests {
     :- Need(HexStrings.IsLooseHexString(algorithmSuiteHex), "Not hex encoded binnary");
     var binaryId := HexStrings.FromHexString(algorithmSuiteHex);
     var algorithmSuite :- AlgorithmSuites
-      .GetAlgorithmSuiteInfo(binaryId)
-      .MapFailure(e => "Invalid Suite:" + algorithmSuiteHex);
+                          .GetAlgorithmSuiteInfo(binaryId)
+                          .MapFailure(e => "Invalid Suite:" + algorithmSuiteHex);
 
     var keysAsStrings := GetArrayString("requiredEncryptionContextKeys", obj).ToOption();
     var requiredEncryptionContextKeys :- if keysAsStrings.Some? then
-        var result := utf8EncodeSeq(keysAsStrings.value);
-        if result.Success? then Success(Some(result.value)) else Failure(result.error)
-      else Success(None);
+                                           var result := utf8EncodeSeq(keysAsStrings.value);
+                                           if result.Success? then Success(Some(result.value)) else Failure(result.error)
+                                         else Success(None);
 
     // TODO fix me
     var commitmentPolicy := CompleteVectors.GetCompatableCommitmentPolicy(algorithmSuite);
     var maxPlaintextLength := None; // GetString("maxPlaintextLength", obj);
-    
-    match typ
-      case "positive-keyring" =>
-        var encryptKeyDescriptionObject :- Get("encryptKeyDescription", obj);
-        var decryptKeyDescriptionObject :- Get("decryptKeyDescription", obj);
-
-        var encryptKeyDescription :- ToKeyDescription(encryptKeyDescriptionObject);
-        var decryptKeyDescription :- ToKeyDescription(decryptKeyDescriptionObject);
-
-        var encryptInfo :- ToKeyringInfo(keys, encryptKeyDescription);
-        var decryptInfo :- ToKeyringInfo(keys, decryptKeyDescription);
-
-        Success(PositiveEncryptKeyringVector(
-          name := name,
-          description := description,
-          encryptionContext := encryptionContext,
-          commitmentPolicy := commitmentPolicy,
-          algorithmSuite := algorithmSuite,
-          maxPlaintextLength := maxPlaintextLength,
-          requiredEncryptionContextKeys := requiredEncryptionContextKeys,
-          keyringInfos := PositiveKeyringInfo(encryptInfo, decryptInfo)
-        ))
-      case "negative-keyring" =>
-        var keyDescriptionObject :- Get("keyDescription", obj);
-        var keyDescription :- ToKeyDescription(keyDescriptionObject);
-        var keyringInfo :- ToKeyringInfo(keys, keyDescription);
-
-        var errorDescription :- GetString("errorDescription", obj);
-        Success(NegativeEncryptKeyringVector(
-          name := name,
-          description := description,
-          encryptionContext := encryptionContext,
-          commitmentPolicy := commitmentPolicy,
-          algorithmSuite := algorithmSuite,
-          maxPlaintextLength := maxPlaintextLength,
-          requiredEncryptionContextKeys := requiredEncryptionContextKeys,
-          errorDescription := errorDescription,
-          keyringInfo := keyringInfo
-        ))
-      case _ => Failure("Unsupported EncryptTestVector type:" + typ)
-  }
-
-  function ToKeyDescription(obj: JSON): Result<KeyDescription, string>
-  {
-    :- Need(obj.Object?, "KeyDescription not an object");
-    var obj := obj.obj;
-    var typString := "type";
-    var typ :- GetString(typString, obj);
-
-    :- Need(TestVectors.KeyDescriptionString?(typ), "Unsupported KeyDescription type:" + typ);
-    var key :- GetString("key", obj);
 
     match typ
-      case "invalid" =>
-        Success(InvalidKeyring(key))
-      case "aws-kms" =>
-        Success(KMSInfo(key))
-      case "aws-kms-mrk-aware" =>
-        Success(KmsMrkAware(key))
-      case "aws-kms-mrk-aware-discovery" =>
-        var defaultMrkRegion :- GetString("partition", obj);
-        var filter := GetObject("aws-kms-discovery-filter", obj);
-        var awsKmsDiscoveryFilter := ToDiscoveryFilter(obj);
-        Success(KmsMrkAwareDiscovery(
-          defaultMrkRegion := defaultMrkRegion,
-          awsKmsDiscoveryFilter := awsKmsDiscoveryFilter
-        ))
-      case "raw" =>
-        var algorithm :- GetString("encryption-algorithm", obj);
-        var providerId :- GetString("provider-id", obj);
-        :- Need(TestVectors.RawAlgorithmString?(algorithm), "Unsupported algorithm:" + algorithm);
-        match algorithm
-          case "aes" =>
-            Success(RawAES(key, providerId))
-          case "rsa" =>
-            var paddingAlgorithm :- GetString("padding-algorithm", obj);
-            var paddingHash :- GetString("padding-hash", obj);
-            :- Need(TestVectors.PaddingAlgorithmString?(paddingAlgorithm), "Unsupported paddingAlgorithm:" + paddingAlgorithm);
-            :- Need(TestVectors.PaddingHashString?(paddingHash), "Unsupported paddingHash:" + paddingHash);
+    case "positive-keyring" =>
+      var encryptKeyDescriptionObject :- Get("encryptKeyDescription", obj);
+      var decryptKeyDescriptionObject :- Get("decryptKeyDescription", obj);
 
-            match paddingAlgorithm
-              case "pkcs1" => 
-                :- Need(paddingHash == "sha1", "Unsupported padding with pkcs1:" + paddingHash);
-                Success(RawRSA(key, providerId, Types.PKCS1))
-              case "oaep-mgf1" => match paddingHash
-                case "sha1" => Success(RawRSA(key, providerId, Types.OAEP_SHA1_MGF1))
-                case "sha256" => Success(RawRSA(key, providerId, Types.OAEP_SHA256_MGF1))
-                case "sha384" => Success(RawRSA(key, providerId, Types.OAEP_SHA384_MGF1))
-                case "sha512" => Success(RawRSA(key, providerId, Types.OAEP_SHA512_MGF1))
+      // Be nice if `document` mapped to `JSON.AST.JSON`
+      var encryptStr :- API.Serialize(encryptKeyDescriptionObject).MapFailure(e => "Whoops");
+      var decryptStr :- API.Serialize(decryptKeyDescriptionObject).MapFailure(e => "Whoops");
+      var encryptKeyDescription :- keys
+                                   .GetKeyDescription(KeyVectorsTypes.GetKeyDescriptionInput(
+                                                        json := encryptStr
+                                                      ))
+                                   .MapFailure(e => "Whoops");
+      var decryptKeyDescription :- keys
+                                   .GetKeyDescription(KeyVectorsTypes.GetKeyDescriptionInput(
+                                                        json := decryptStr
+                                                      ))
+                                   .MapFailure(e => "Whoops");
+
+      Success(PositiveEncryptKeyringVector(
+                name := name,
+                description := description,
+                encryptionContext := encryptionContext,
+                commitmentPolicy := commitmentPolicy,
+                algorithmSuite := algorithmSuite,
+                maxPlaintextLength := maxPlaintextLength,
+                requiredEncryptionContextKeys := requiredEncryptionContextKeys,
+                encryptDescription := encryptKeyDescription.keyDescription,
+                decryptDescription := decryptKeyDescription.keyDescription
+              ))
+    case "negative-keyring" =>
+      var keyDescriptionObject :- Get("keyDescription", obj);
+      var keyStr :- API.Serialize(keyDescriptionObject).MapFailure(e => "Whoops");
+      var keyDescription :- keys
+                            .GetKeyDescription(KeyVectorsTypes.GetKeyDescriptionInput(
+                                                 json := keyStr
+                                               ))
+                            .MapFailure(e => "Whoops");
+
+      var errorDescription :- GetString("errorDescription", obj);
+      Success(NegativeEncryptKeyringVector(
+                name := name,
+                description := description,
+                encryptionContext := encryptionContext,
+                commitmentPolicy := commitmentPolicy,
+                algorithmSuite := algorithmSuite,
+                maxPlaintextLength := maxPlaintextLength,
+                requiredEncryptionContextKeys := requiredEncryptionContextKeys,
+                errorDescription := errorDescription,
+                keyDescription := keyDescription.keyDescription
+              ))
+    case _ => Failure("Unsupported EncryptTestVector type:" + typ)
   }
-
-  function ToKeyringInfo(keys: map<string, KeyMaterial>,  description: KeyDescription)
-    : Result<KeyringInfo, string>
-  {
-    var material :- match description
-      case KmsMrkAwareDiscovery(_, _) => Success(None)
-      case _ => 
-      :- Need(description.key in keys, "Key does not exist:" + description.key);
-      Success(Some(keys[description.key]));
-    Success(KeyringInfo(description, material))
-  }
-
-  function ToDiscoveryFilter(obj: seq<(string, JSON)>) : Option<Types.DiscoveryFilter>
-  {
-    var filter :- GetObject("aws-kms-discovery-filter", obj).ToOption();
-    var partition :- GetString("partition", filter).ToOption();
-    var accountIds :- GetArrayString("account-ids", filter).ToOption();
-    Some(Types.DiscoveryFilter(
-      partition := partition,
-      accountIds := accountIds
-    ))
-  }
-
-  function ToEncryptedDataKey(obj: seq<(string, JSON)>)
-    : Result<Types.EncryptedDataKey, string>
-  {
-    var keyProviderIdJSON :- GetString("keyProviderId", obj);
-    var keyProviderInfoJSON :- GetString("keyProviderInfo", obj);
-    var ciphertextJSON :- GetString("ciphertext", obj);
-
-    var keyProviderId :- UTF8.Encode(keyProviderIdJSON);
-    var keyProviderInfo :- Base64.Decode(keyProviderInfoJSON);
-    var ciphertext :- Base64.Decode(ciphertextJSON);
-
-    Success(Types.EncryptedDataKey(
-      keyProviderId := keyProviderId,
-      keyProviderInfo := keyProviderInfo,
-      ciphertext := ciphertext
-    ))
-  }
-
-  function utf8EncodePair(key: string, value: string):
-    (res: Result<(UTF8.ValidUTF8Bytes, UTF8.ValidUTF8Bytes), string>)
-  {
-    var utf8Key :- UTF8.Encode(key);
-    var utf8Value :- UTF8.Encode(value);
-
-    Success((utf8Key, utf8Value))
-  }
-
-    // TODO: These EncryptionContext methods can be removed once we move to UTF8 strings
-  function utf8EncodeMap(mapStringString: map<string, string>):
-    (res: Result<Types.EncryptionContext, string>)
-  {
-    if |mapStringString| == 0 then
-      Success(map[])
-    else
-
-      var encodedResults := map key <- mapStringString :: key := utf8EncodePair(key, mapStringString[key]);
-      :- Need(forall r <- encodedResults.Values :: r.Success?, "String can not be UTF8 Encoded?");
-
-      Success(map r <- encodedResults.Values :: r.value.0 := r.value.1)
-  }
-
-  function utf8EncodeSeq(seqOfStrings: seq<string>)
-    :(res: Result<seq<Types.Utf8Bytes>, string>)
-  {
-    var encodedResults := seq(|seqOfStrings|, i requires 0 <= i < |seqOfStrings| => UTF8.Encode(seqOfStrings[i]));
-    :- Need(forall r <- encodedResults :: r.Success?, "String can not be UTF8 Encoded?");
-    Success(seq(|encodedResults|, i requires 0 <= i < |encodedResults| => encodedResults[i].value))
-  }
-
 }
